src/Init/Data/Iterators/Consumers/Loop.lean
@@ -137,6 +137,14 @@ def Iter.Partial.size {α : Type w} {β : Type w} [Iterator α Id β] [IteratorS
     (it : Iter (α := α) β) : Nat :=
   (IteratorSizePartial.size it.toIterM).run.down
 
+/--
+`LawfulIteratorSize α m` ensures that the `size` function of an iterator behaves as if it
+iterated over the whole iterator, counting its elements and causing all the monadic side effects
+of the iterations. This is a fairly strong condition for monadic iterators and it will be false
+for many efficient implementations of `size` that compute the size without actually iterating.
+
+This class is experimental and users of the iterator API should not explicitly depend on it.
+-/
 class LawfulIteratorSize (α : Type w) {β : Type w} [Iterator α Id β] [Finite α Id]
     [IteratorSize α Id] where
     size_eq_size_toArray {it : Iter (α := α) β} : it.size =
