src/Init/Data/Range/Polymorphic/RangeIterator.lean
@@ -277,7 +277,7 @@ instance RangeIterator.instIteratorAccess [UpwardEnumerable α] [SupportsUpperBo
         .done, (by
       induction n generalizing it
       · split <;> rename_i heq
-        · apply IterM.IsPlausibleNthOutput.done
+        · apply IterM.IsPlausibleNthOutputStep.done
           simp only [Monadic.isPlausibleStep_iff, Monadic.step]
           simp only [Option.bind_eq_none_iff, UpwardEnumerable.succMany?_zero, reduceCtorEq,
             imp_false] at heq
@@ -291,26 +291,26 @@ instance RangeIterator.instIteratorAccess [UpwardEnumerable α] [SupportsUpperBo
           simp only [heq', Option.bind_some, UpwardEnumerable.succMany?_zero, Option.some.injEq] at heq
           cases heq
           split <;> rename_i heq''
-          · apply IterM.IsPlausibleNthOutput.zero_yield
+          · apply IterM.IsPlausibleNthOutputStep.zero_yield
             simp [Monadic.isPlausibleStep_iff, Monadic.step, heq', heq'']
-          · apply IterM.IsPlausibleNthOutput.done
+          · apply IterM.IsPlausibleNthOutputStep.done
             simp [Monadic.isPlausibleStep_iff, Monadic.step, heq', heq'']
       · rename_i n ih
         split <;> rename_i heq
         · cases heq' : it.internalState.next
-          · apply IterM.IsPlausibleNthOutput.done
+          · apply IterM.IsPlausibleNthOutputStep.done
             simp only [Monadic.isPlausibleStep_iff, Monadic.step, heq']
           · rename_i out
             simp only [heq', Option.bind_some, LawfulUpwardEnumerable.succMany?_succ_eq_succ_bind_succMany] at heq
             specialize ih ⟨⟨UpwardEnumerable.succ? out, it.internalState.upperBound⟩⟩
             simp only [heq] at ih
             by_cases heq'' : SupportsUpperBound.IsSatisfied it.internalState.upperBound out
-            · apply IterM.IsPlausibleNthOutput.yield
+            · apply IterM.IsPlausibleNthOutputStep.yield
               · simp only [Monadic.isPlausibleStep_iff, Monadic.step, heq', heq'', ↓reduceIte,
                 IterStep.yield.injEq]
                 exact ⟨rfl, rfl⟩
               · exact ih
-            · apply IterM.IsPlausibleNthOutput.done
+            · apply IterM.IsPlausibleNthOutputStep.done
               simp [Monadic.isPlausibleStep_iff, Monadic.step, heq', heq'']
         · cases heq' : it.internalState.next
           · simp [heq'] at heq
@@ -321,7 +321,7 @@ instance RangeIterator.instIteratorAccess [UpwardEnumerable α] [SupportsUpperBo
           specialize ih ⟨⟨UpwardEnumerable.succ? out, it.internalState.upperBound⟩⟩
           simp only [heq] at ih
           by_cases hout : SupportsUpperBound.IsSatisfied it.internalState.upperBound out
-          · apply IterM.IsPlausibleNthOutput.yield
+          · apply IterM.IsPlausibleNthOutputStep.yield
             · simp only [Monadic.isPlausibleStep_iff, Monadic.step, heq', hout, ↓reduceIte,
               IterStep.yield.injEq]
               exact ⟨rfl, rfl⟩
@@ -329,7 +329,7 @@ instance RangeIterator.instIteratorAccess [UpwardEnumerable α] [SupportsUpperBo
           · have := hout.imp (fun h => LawfulUpwardEnumerableUpperBound.isSatisfied_of_le _ _ _ h hle)
             simp only [this, ↓reduceIte]
             simp only [this, ↓reduceIte] at ih
-            apply IterM.IsPlausibleNthOutput.done
+            apply IterM.IsPlausibleNthOutputStep.done
             simp [Monadic.isPlausibleStep_iff, Monadic.step, heq', hout])⟩
 
 instance RangeIterator.instLawfulDeterministicIterator [UpwardEnumerable α] [SupportsUpperBound su α]
